wip

src/tactic/hammer/monomorphization.lean
@@ -1,16 +1,92 @@
-import data.analysis.filter
+import tactic.core
 tactic.hammer.fo_translation
+super
 
-meta def expr.consts_and_local_consts (e : expr) : list expr :=
-native.rb_set.to_list $ e.fold native.mk_rb_set $ λ e _ s,
-match e with
-| e@(expr.const n _) := s.insert n
-| _ := s
+local attribute [inline] decidable.to_bool bool.decidable_eq
+option.decidable_exists_mem
+
+open native
+
+meta def list.dup_native {α} [has_lt α] [decidable_rel ((<) : α → α → Prop)] (xs : list α) : list α :=
+rb_set.to_list $ rb_map.set_of_list xs
+
+meta def list.group_by_native {α β} [has_lt α] [decidable_rel ((<) : α → α → Prop)] (xs : list β) (f : β → α) : rb_map α (list β) :=
+xs.foldl (λ m x, m.insert (f x) (x :: (m.find (f x)).get_or_else [])) mk_rb_map
+
+open expr
+
+meta def expr.app_short (a b : expr) : expr :=
+match a with
+| (lam _ _ _ a) := a.instantiate_var b
+| _ := app a b
 end
+
+meta def level.has_mvar : level → bool
+| (level.param _) := ff
+| (level.succ l) := l.has_mvar
+| (level.mvar _) := tt
+| level.zero := ff
+| (level.max l1 l2) := l1.has_mvar ∨ l2.has_mvar
+| (level.imax l1 l2) := l1.has_mvar ∨ l2.has_mvar
+
+meta def expr.has_level_mvar : expr → bool
+| (var _) := ff
+| (mvar _ _ t) := t.has_level_mvar
+| (sort l) := l.has_mvar
+| (macro _ es) := es.any expr.has_level_mvar
+| (app a b) := a.has_level_mvar ∨ b.has_level_mvar
+| (expr.const _ ls) := ls.any level.has_mvar
+| (expr.local_const _ _ _ t) := t.has_level_mvar
+| (pi _ _ a b) := a.has_level_mvar ∨ b.has_level_mvar
+| (lam _ _ a b) := a.has_level_mvar ∨ b.has_level_mvar
+| (elet _ a b c) := a.has_level_mvar ∨ b.has_level_mvar ∨ c.has_level_mvar
+
+meta def expr.consts_and_local_consts_core : expr → rb_set expr → rb_set expr
+| (var _) := id
+| (mvar _ _ _) := id
+| (sort _) := id
+| (macro _ es) := λ s, es.foldl (λ s e, e.consts_and_local_consts_core s) s
+| (app a b) := a.consts_and_local_consts_core ∘ b.consts_and_local_consts_core
+| e@(expr.const _ _) := if e.has_level_mvar then id else λ s, s.insert e
+| e@(expr.local_const _ _ _ t) := if t.has_var ∨ t.has_level_mvar then id else λ s, s.insert e
+| (pi _ _ a b) := a.consts_and_local_consts_core ∘ b.consts_and_local_consts_core
+| (lam _ _ a b) := a.consts_and_local_consts_core ∘ b.consts_and_local_consts_core
+| (elet _ a b c) :=
+  a.consts_and_local_consts_core ∘ b.consts_and_local_consts_core
+    ∘ c.consts_and_local_consts_core
+
+meta def consts_and_local_consts (es : list expr) : list expr :=
+rb_set.to_list $ es.foldl (λ s e, e.consts_and_local_consts_core s) mk_rb_set
+
+meta def tactic.retrieve_or_else {α} (a : α) (tac : tactic α) : tactic α :=
+λ s, result.cases_on (tac s)
+  (λ a _, result.success a s)
+  (λ _ _ _, result.success a s)
+
+meta def tactic.collect_successes {α β} (as : list α) (tac : α → tactic (list β)) : tactic (list β) :=
+list.join <$> as.mmap (λ a, tactic.retrieve_or_else [] (tac a))
+
+meta def mk_lam (lc : expr) (e : expr) : expr :=
+expr.lam lc.local_pp_name lc.local_binding_info lc.local_type (e.abstract_local lc.local_uniq_name)
 
 namespace hammer
 
 open expr tactic
+
+meta def get_head_name : expr → name
+| (app a _) := get_head_name a
+| (local_const _ uniq_name _ _) := uniq_name
+| (const n _) := n
+| _ := name.anonymous
+
+meta def hint_name : expr → name
+| (app a _) := hint_name a
+| (lam _ _ _ a) := hint_name a
+| (local_const _ (name.mk_string n _) _ _) := n
+| (local_const un (name.mk_numeral _ n) bi t) := hint_name (local_const un n bi t)
+| (const (name.mk_string n _) _) := n
+| (const _ _) := `c
+| _ := `x
 
 meta def num_mono_args : expr → ℕ
 | (expr.pi pp_n bi d t) :=
@@ -23,4 +99,475 @@ meta def num_mono_args : expr → ℕ
     0
 | _ := 0
 
+#eval (num_mono_args <$> infer_type `(@has_add.add.{0})) >>= trace
+
+meta def gather_constant_heads (nargs : rb_map name ℕ) : expr → list expr
+| (lam _ _ d e) := gather_constant_heads d ++ gather_constant_heads e
+| (pi _ _ d e) := gather_constant_heads d ++ gather_constant_heads e
+| (elet _ a b c) := gather_constant_heads a ++ gather_constant_heads b ++ gather_constant_heads c
+| e :=
+let fn := e.get_app_fn, as := e.get_app_args in
+let acc := if as = [] then [] else gather_constant_heads fn ++ as.bind gather_constant_heads in
+match nargs.find (get_head_name fn) with
+| some n :=
+  let ch := mk_app fn (as.take n) in
+  if n ≤ as.length ∧ ¬ ch.has_var then ch :: acc else acc
+| none := acc
+end
+
+meta def monom_core {α} (nargs : rb_map name ℕ) (cheads : rb_map name (list expr)) :
+  expr → tactic (list α) → tactic (list α)
+| (lam _ _ d e) cont := monom_core d $ monom_core e $ cont
+| (pi _ _ d e) cont := monom_core d $ monom_core e $ cont
+| (elet _ a b c) cont := monom_core a $ monom_core b $ monom_core c $ cont
+| e cont :=
+-- if ¬ e.has_meta_var ∧ ¬ e.has_level_mvar then cont else
+let fn := e.get_app_fn, fnn := get_head_name fn, as := e.get_app_args in
+-- do trace fn, trace nargs, trace cheads,
+match (nargs.find fnn, cheads.find fnn) with
+| (some n, some chs) := do
+  e' ← instantiate_mvars $ mk_app fn (as.take n),
+  -- trace (e, n, chs),
+  if ¬ e'.has_meta_var ∧ ¬ e'.has_level_mvar then
+    (as.drop n).foldl (λ cont a, monom_core a cont) cont
+  else do
+    res1 ← (collect_successes chs $ λ ch, do
+      -- trace (ch, e'),
+      unify ch e',
+      (as.drop n).foldl (λ cont a, monom_core a cont) cont),
+    -- trace res1.length,
+    res2 ← retrieve_or_else [] $
+      (as.drop n).foldl (λ cont a, monom_core a cont) cont,
+    pure $ res1 ++ res2
+| _ :=
+  if as = [] then cont else
+  (fn :: as : list expr).foldl (λ cont a, monom_core a cont) cont
+end
+
+meta def monom' (nargs : rb_map name ℕ) (cheads : rb_map name (list expr)) :
+  expr → expr → (expr → tactic expr) → tactic (list expr)
+| (pi n bi d ty) prf cont := do
+  m ← mk_meta_var d,
+  monom' (ty.instantiate_var m) (prf.app_short m) $ λ prf, do
+    try $ mk_instance d >>= unify m,
+    m ← instantiate_mvars m,
+    match m with
+    | (mvar _ _ _) := do
+      l ← mk_local' n bi d,
+      unify m l,
+      prf ← instantiate_mvars prf,
+      cont $ mk_lam l prf
+    | _ := cont prf
+    end
+| ty prf cont :=
+-- do trace ty,
+  monom_core nargs cheads ty $ (λ x, [x]) <$> cont prf
+
+meta def monom (nargs : rb_map name ℕ) (cheads : rb_map name (list expr))
+  (prf : expr) : tactic (list expr) := do
+ty ← infer_type prf,
+retrieve_or_else [] $
+monom' nargs cheads ty prf $ λ prf, do
+prf ← instantiate_mvars prf,
+guard $ ¬ prf.has_meta_var,
+guard $ ¬ prf.has_level_mvar,
+pure prf
+
+meta def monomorphization_round (lems : list expr) : tactic (list expr) := do
+cs ← _root_.consts_and_local_consts <$> lems.mmap infer_type,
+-- trace cs,
+nargs ← rb_map.of_list <$> cs.mmap (λ c, do t ← infer_type c, pure (get_head_name c, num_mono_args t)),
+-- trace nargs,
+cheads ← lems.mmap (λ lem, gather_constant_heads nargs <$> infer_type lem),
+let cheads := (cheads.join.group_by_native get_head_name).map list.dup_native,
+-- trace cheads,
+lems' ← lems.mmap $ λ lem, monom nargs cheads lem,
+lems' ← lems'.join.mmap (λ lem, do t ← infer_type lem, pure (t, lem)),
+let lems' := (lems'.group_by_native prod.fst).to_list.map (λ ⟨k, vs⟩, vs.head.2),
+let lems' := lems'.dup_native,
+-- trace lems',
+-- lems'.mmap infer_type >>= trace,
+pure lems'
+
+meta def monomorphize (lems : list expr) (rounds := 2) : tactic (list expr) :=
+rounds.iterate (λ lems', do lems' ← lems', monomorphization_round (lems ++ lems')) (pure [])
+
+meta structure intern_state :=
+(fresh_idx : ℕ := 0)
+(nfs : list expr := [])
+(nargs : rb_map name ℕ)
+
+@[reducible]
+meta def intern := state_t intern_state tactic
+
+meta def tactic_mfind {α} (tac : α → tactic unit) : list α → tactic α
+| [] := failed
+| (h::t) := tac h >> return h <|> tactic_mfind t
+
+meta def intern.fresh_num : intern ℕ := do
+state_t.modify (λ s, { fresh_idx := s.fresh_idx + 1, ..s }),
+intern_state.fresh_idx <$> state_t.get
+
+meta def intern.fresh_name (hint : name) : intern name :=
+do n ← intern.fresh_num, pure $ name.mk_numeral (unsigned.of_nat n) hint
+
+meta def intern_here : ∀ (lctx : list expr) (e : expr), intern expr
+| _ e@(const _ []) := pure e
+| _ e@(local_const _ _ _ _) := pure e
+| (lc :: lctx) e :=
+  let e' := e.abstract_local lc.local_uniq_name in
+  if ¬ e'.has_var then intern_here lctx e else do
+  e'' ← intern_here lctx (lam lc.local_pp_name binder_info.default lc.local_type e'),
+  -- this is wrong
+  pure (e'' lc)
+| [] e := do
+  nfs ← intern_state.nfs <$> state_t.get,
+  nf ← state_t.lift $ try_core $ first $ nfs.map (λ nf, do is_def_eq e nf, pure nf),
+  match nf with
+  | some nf := pure nf
+  | _ := do
+    n ← intern.fresh_name (hint_name e),
+    -- state_t.lift $ trace (n,e),
+    c ← state_t.lift $ pose n none e,
+    state_t.modify $ λ st, { nfs := c :: nfs, ..st },
+    pure c
+  end
+
+meta def get_nargs (e : expr) : intern (option ℕ) := do
+nargs ← intern_state.nargs <$> state_t.get,
+pure (nargs.find (get_head_name e))
+
+meta def intern_ty (lctx : list expr) : expr → intern expr
+| t@(sort _) := pure t
+| e@(pi pp_n bi d t) :=
+  if t.has_var then intern_here [] e else
+  imp <$> intern_ty d <*> intern_ty t
+| e := intern_here lctx e
+
+meta def intern_expr : list expr → expr → intern expr
+| lctx `(%%a = %%b) := do
+  a ← intern_expr lctx a,
+  b ← intern_expr lctx b,
+  state_t.lift $ mk_app ``eq [a,b]
+| lctx `(@Exists %%α %%p@(lam _ _ _ _)) := do
+  α ← intern_ty lctx α,
+  p ← intern_expr lctx p,
+  state_t.lift $ mk_mapp ``Exists [α, p]
+| lctx (app (app (const ``Exists ls) α) p) :=
+  -- η-expand
+  intern_expr lctx (app (const ``Exists ls)
+    α (lam `x binder_info.default α (p (var 0))))
+| lctx e@(app a b) := do
+  nargs ← get_nargs e,
+  if ∃ n ∈ nargs, n ≥ e.get_app_num_args then intern_here lctx e else do
+  ta ← state_t.lift $ infer_type a >>= whnf,
+  let is_dep := match ta with
+    | (expr.pi _ _ _ t) := t.has_var
+    | _ := tt
+    end,
+  if is_dep then intern_here lctx e else app <$> intern_expr lctx a <*> intern_expr lctx b
+| lctx e@(pi pp_n bi d t0) := do
+  lc ← state_t.lift $ mk_local' pp_n bi d,
+  let t := t0.instantiate_var lc,
+  t_prop ← state_t.lift $ is_prop t,
+  d_prop ← state_t.lift $ is_prop d,
+  if ¬ t_prop then intern_here lctx e
+  else if d_prop ∧ ¬ t0.has_var then -- implication
+    imp <$> intern_expr lctx d <*> intern_expr lctx t
+  else do -- forall
+    d ← intern_ty lctx d,
+    t ← intern_expr (lc :: lctx) t,
+    pure (pi pp_n binder_info.default d (t.abstract_local lc.local_uniq_name))
+| lctx e@(lam pp_n bi d t) := do
+  lc ← state_t.lift $ mk_local' pp_n bi d,
+  let t := t.instantiate_var lc,
+  -- t_prop ← state_t.lift $ is_prop t,
+  -- if ¬ t_prop then intern_here lctx e else do
+  d ← intern_ty lctx d,
+  t ← intern_expr (lc :: lctx) t,
+  pure (lam pp_n binder_info.default d (t.abstract_local lc.local_uniq_name))
+| lctx e := intern_here lctx e
+
+meta def intern_lems (lems : list expr) : tactic (list (expr × expr)) := do
+tys ← lems.mmap infer_type,
+let cs := _root_.consts_and_local_consts tys,
+-- trace cs,
+nargs ← rb_map.of_list <$> cs.mmap (λ c, do t ← infer_type c, pure (get_head_name c, num_mono_args t)),
+(tys', st) ← state_t.run (lems.mmap (λ l,
+  do t ← state_t.lift (infer_type l), t ← intern_expr [] t, pure (l, t))) { nargs := nargs },
+pure tys'
+
+meta def tptpify_quant' (q : string) (x : string) (t : format) (b : format) : format :=
+format.paren' $ q ++ (format.nest 1 $ format.group $
+  "[" ++ x ++ ":" ++ format.line ++ t ++ "]:") ++ format.line ++ b
+
+meta structure to_tf0_state :=
+(fresh_idx := 0)
+(ns : rb_map expr string := mk_rb_map)
+
+@[reducible] meta def to_tf0 := state_t to_tf0_state tactic
+
+meta def to_tf0.name_core (e : expr) (f : name → string) : to_tf0 string := do
+ns ← to_tf0_state.ns <$> state_t.get,
+match ns.find e with
+| some n := pure n
+| none := do
+  state_t.modify $ λ st, { fresh_idx := st.fresh_idx + 1, ..st },
+  idx ← to_tf0_state.fresh_idx <$> state_t.get,
+  let n := match e with
+    | (const n _) := f n
+    | _ := f (name.mk_numeral (unsigned.of_nat idx) (hint_name e))
+    end,
+  state_t.modify $ λ st, { ns := st.ns.insert e n, ..st },
+  pure n
+end
+
+meta def to_tf0.var_name (e : expr) : to_tf0 string :=
+to_tf0.name_core e var_tptpify_name
+
+meta def to_tf0.con_name (e : expr) : to_tf0 string :=
+to_tf0.name_core e fn_tptpify_name
+
+meta def to_tf0.ax_name (e : expr) : to_tf0 string :=
+to_tf0.name_core e ax_tptpify_name
+
+meta mutual def to_tf0_ty, to_tf0_ty_fun
+with to_tf0_ty : expr → to_tf0 format
+| (sort level.zero) := pure "$o"
+| lc@(local_const _ _ _ _) :=
+  format.of_string <$> to_tf0.con_name lc
+| c@(const n _) := format.of_string <$> to_tf0.con_name c
+| e@(pi _ _ _ _) := format.paren' <$> to_tf0_ty_fun e
+| e := do state_t.lift $ trace e, pure "e_UNSUPPORTED"
+with to_tf0_ty_fun : expr → to_tf0 format
+| (pi _ _ a b) := do
+  a' ← to_tf0_ty a,
+  b' ← to_tf0_ty_fun b,
+  pure $ a' ++ format.space ++ ">" ++ format.line ++ b'
+| a := to_tf0_ty a
+
+meta def to_tf0_tm : list expr → expr → to_tf0 format
+| lctx lc@(local_const _ _ _ _) :=
+  format.of_string <$> if lc ∈ lctx then to_tf0.var_name lc else to_tf0.con_name lc
+| lctx (const n _) := pure $ fn_tptpify_name n
+| lctx `(%%x = %%y) := tptpify_binop "=" <$> to_tf0_tm lctx x <*> to_tf0_tm lctx y
+| lctx `(%%x ∧ %%y) := tptpify_binop "&" <$> to_tf0_tm lctx x <*> to_tf0_tm lctx y
+| lctx `(%%x ∨ %%y) := tptpify_binop "|" <$> to_tf0_tm lctx x <*> to_tf0_tm lctx y
+| lctx `(%%x ↔ %%y) := tptpify_binop "<=>" <$> to_tf0_tm lctx x <*> to_tf0_tm lctx y
+| lctx `(¬ %%x) := do
+  x' ← to_tf0_tm lctx x,
+  pure $ format.paren' $ "~" ++ format.line ++ x'
+| lctx (app (app (const ``Exists _) _) (lam pp_n _ d a)) := do
+  lc ← state_t.lift $ mk_local' pp_n binder_info.default d,
+  tptpify_quant' "?" <$> to_tf0.var_name lc <*> to_tf0_ty d <*>
+    to_tf0_tm (lc :: lctx) (a.instantiate_var lc)
+| lctx e@(pi pp_n _ d a) := do
+  d_is_prop ← state_t.lift $ is_prop d,
+  if ¬ d_is_prop then do
+    lc ← state_t.lift $ mk_local' pp_n binder_info.default d,
+    let a' := a.instantiate_var lc,
+    tptpify_quant' "!" <$> to_tf0.var_name lc <*> to_tf0_ty d <*> to_tf0_tm (lc :: lctx) a'
+  else
+    if a.has_var then do
+      state_t.lift $ trace e, pure "e_UNSUPPORTED"
+    else
+      tptpify_binop "=>" <$> to_tf0_tm lctx d <*> to_tf0_tm lctx a
+| lctx e@(app _ _) :=
+  let fn := e.get_app_fn, as := e.get_app_args in
+  (format.paren' ∘ format.join ∘ list.intersperse (format.space ++ "@" ++ format.line))
+    <$> (fn :: as).mmap (to_tf0_tm lctx)
+-- | lctx (app a b) := tptpify_binop "@" <$> to_tf0_tm lctx a <*> to_tf0_tm lctx b
+| _ e := do state_t.lift $ trace e, pure "e_UNSUPPORTED"
+
+meta def to_tf0.run {α} (t : to_tf0 α) : tactic α :=
+prod.fst <$> state_t.run t {}
+
+meta def tptpify_thf_ann (role : string) (n : string) (f : format) : format :=
+format.group $ format.nest 1 $ "thf(" ++ format.group (
+    n ++ "," ++ format.line ++ role ++ ",")
+  ++ format.line ++ f ++ ")."
+
+meta def to_tf0_file (lems : list (expr × expr)) : to_tf0 (format × list (string × expr × expr)) := do
+lems ← lems.mfilter (λ ⟨pr, ty⟩, state_t.lift $ is_prop ty),
+let cs := (_root_.consts_and_local_consts (lems.map prod.snd)).filter
+  (λ c, c.const_name ≠ ``eq ∧ c.const_name ≠ ``Exists),
+sorts ← cs.mfilter (λ c, do t ← state_t.lift $ infer_type c >>= whnf,
+  pure $ match t with
+  | (sort level.zero) := ff
+  | (sort _) := tt
+  | _ := ff
+  end),
+sort_decls ← sorts.mmap (λ c, do
+  c' ← to_tf0.con_name c,
+  pure $ tptpify_thf_ann "type" ("ty_" ++ c')
+    (tptpify_binop ":" c' "$tType")),
+cs ← cs.mfilter (λ c, do t ← state_t.lift $ infer_type c >>= whnf,
+  pure $ match t with
+  | (sort level.zero) := tt
+  | (sort _) := ff
+  | _ := tt
+  end),
+ty_decls ← cs.mmap (λ c, do
+  t ← state_t.lift $ infer_type c,
+  t' ← to_tf0_ty t,
+  c' ← to_tf0.con_name c,
+  pure $ tptpify_thf_ann "type" ("ty_" ++ c') (tptpify_binop ":" c' t')),
+axs ← lems.mmap (λ ⟨pr, ty⟩, do
+  n ← to_tf0.ax_name pr,
+  ann ← tptpify_thf_ann "axiom" n <$> to_tf0_tm [] ty,
+  pure (n, pr, ty, ann)),
+let tptp := format.join $ (sort_decls ++ ty_decls ++ axs.map (λ ⟨n,pr,ty,ann⟩, ann))
+  .intersperse (format.line ++ format.line),
+pure (tptp, axs.map (λ ⟨n,pr,ty,ann⟩, (n, pr, ty)))
+
+meta def get_head_const : expr → expr
+| (app a b) := get_head_const a
+| a@(lam _ _ _ b) := if b.has_var then a else get_head_const b
+| e := e
+
+meta def mk_monom_file (axs : list name) : tactic (format × list (string × expr × expr)) := do
+goal ← retrieve (revert_all >> target),
+let axs := goal.constants.filter is_good_const ++ axs,
+axs ← close_under_references axs,
+-- trace $ (axs.map name.to_string).qsort (λ a b, a < b),
+repeat (intro1 >> skip),
+(do tgt ← target, when (tgt ≠ `(false)) $
+  mk_mapp ``classical.by_contradiction [some tgt] >>= eapply >> intro1 >> skip),
+lems ← (++) <$> axs.mmap mk_const <*> local_context,
+lems' ← monomorphize lems 2,
+lems'' ← intern_lems lems',
+(to_tf0_file lems'').run
+
+meta def filter_lemmas_via_monom (axs : list name) : tactic (list (expr × expr)) := do
+(tptp, ax_names) ← mk_monom_file axs,
+(tactic.unsafe_run_io $ do f ← io.mk_file_handle "hammer.p" io.mode.write, io.fs.write f tptp.to_string.to_char_buffer, io.fs.close f),
+let ax_names := rb_map.of_list ax_names,
+-- (failure : tactic unit),
+tptp_out ← exec_cmd "bash" ["-c",
+  "set -o pipefail; eprover-ho --cpu-limit=30 --proof-object=1 | " ++
+    "grep -oP '(?<=file\\(..stdin.., ).*?(?=\\))'"]
+  tptp.to_string,
+let ns := tptp_out.split_on '\n',
+pure $ do n ← ns, (ax_names.find n).to_list
+
+meta def find_lemmas_via_monom (max := 10) : tactic (list (expr × expr)) := do
+axs ← timetac "Premise selection took" $ retrieve $
+  revert_all >> target >>= select_for_goal,
+let axs := (axs.take max).map (λ a, a.1),
+-- trace "Premise selection:",
+trace axs,
+timetac "eprover-ho took" $ filter_lemmas_via_monom axs
+
+namespace mysuper
+open super
+
+meta def initial (local_false : expr) (clauses : list clause) : tactic prover_state := do
+after_setup ← (clauses.mmap' (λc : clause,
+  do mk_derived c { priority := score.prio.immediate, in_sos := ff,
+                    age := 0, cost := 0 } >>= add_inferred
+)).run (prover_state.empty local_false),
+return after_setup.2
+
+meta def default_preprocessing : list (prover unit) :=
+[
+clausify_pre,
+clause_normalize_pre,
+factor_dup_lits_pre,
+remove_duplicates_pre,
+refl_r_pre,
+-- diff_constr_eq_l_pre,
+tautology_removal_pre,
+subsumption_interreduction_pre,
+forward_subsumption_pre,
+return ()
+]
+
+meta def mysuper (lemmas : list expr) (os : super.opts) : tactic unit := do
+try_for os.timeout $ with_trim $ do
+as_refutation, local_false ← target,
+clauses ← lemmas.mmap (clause.of_proof local_false),
+initial_state ← initial local_false clauses,
+inf_names ← attribute.get_instances `super.inf,
+infs ← inf_names.mmap $ λn, eval_expr inf_decl (const n []),
+infs ← return $ list.map inf_decl.inf $ list.sort_on inf_decl.prio infs,
+res ← (run_prover_loop selection21 (age_weight_clause_selection 3 4)
+  default_preprocessing infs
+  os.max_iters 0).run initial_state,
+match res with
+| (some empty_clause, st) := apply empty_clause >> skip
+| (none, saturation) := do sat_fmt ← pp saturation,
+                           fail $ to_fmt "saturation:" ++ format.line ++ sat_fmt
+end
+
+end mysuper
+
+meta def reconstruct (axs : list (expr × expr)) : tactic unit := focus1 $ do
+lems ← axs.mmap (λ ⟨pr, ty⟩, mk_mapp ``id [ty, pr]),
+mysuper.mysuper lems {}
+
+-- set_option pp.all true
+example (x y : ℤ) (h : x ∣ y) (h2 : x ≤ y) (h3 : ¬ x + y < 0)
+  (h4 : ∃ i : ℤ, i ≤ i + 1) : true := by do
+ls ← local_context,
+l1 ← mk_const ``add_comm,
+l2 ← mk_const ``le_antisymm,
+l3 ← mk_const ``exists_congr,
+let ls : list expr := l1 :: l2 :: l3 :: ls,
+-- ls ← (λ x, [x]) <$> get_local `h3,
+ls' ← monomorphize ls 3,
+ls'' ← intern_lems ls',
+trace_state,
+trace ls'',
+-- ls''.mmap' (λ l'', (to_tf0_tm [] l''.2).run >>= trace),
+(to_tf0_file ls'').run >>= trace,
+triv
+
+-- example (x y : ℤ) (h : x ∣ y) (h2 : x ≤ y) (h3 : ¬ x + y < 0) : true :=
+-- by feature_search
+
 end hammer
+
+namespace tactic
+namespace interactive
+open interactive interactive.types lean.parser
+
+meta def find_lemmas_via_monom (axs : parse $ optional $ list_of ident) (max_lemmas := 10) : tactic unit := do
+lems ←
+  match axs with
+  | none := hammer.find_lemmas_via_monom max_lemmas
+  | some axs := do
+    axs.mmap' (λ ax, get_decl ax),
+    timetac "eprover-ho took" $
+      hammer.filter_lemmas_via_monom axs
+  end,
+trace "eprover-ho proof uses the following lemmas:",
+lems.mmap' (λ ⟨l, t⟩, do
+  l' ← pp l,
+  -- t ← infer_type l >>= pp,
+  t ← pp t,
+  trace (format.nest 4 $ format.group $ "  " ++ l' ++ " :" ++ format.line ++ t)),
+admit
+
+meta def hammer_via_monom (axs : parse $ optional $ list_of ident) (max_lemmas := 10) : tactic unit := do
+lems ←
+  match axs with
+  | none := hammer.find_lemmas_via_monom max_lemmas
+  | some axs := do
+    axs.mmap' (λ ax, get_decl ax),
+    timetac "eprover-ho took" $
+      hammer.filter_lemmas_via_monom axs
+  end,
+trace "eprover-ho proof uses the following lemmas:",
+lems.mmap' (λ ⟨l, t⟩, do
+  l' ← pp l,
+  -- t ← infer_type l >>= pp,
+  t ← pp t,
+  trace (format.nest 4 $ format.group $ "  " ++ l' ++ " :" ++ format.line ++ t)),
+hammer.reconstruct lems
+
+end interactive
+end tactic
+
+set_option trace.super true
+example (x y : ℤ) : x + y = y + x :=
+by hammer_via_monom
