src/tactic/hammer/mex2.lean
@@ -1,0 +1,9 @@
+import tactic.hammer.monomorphization data.nat.gcd data.real.basic
+
+-- set_option profiler true
+set_option trace.super true
+
+example (x y : ℝ) (h : x < y) : ∃ z : ℚ, x < z ∧ (z : ℝ) ≤ y :=
+by hammer_via_monom 60
+-- by feature_search
+-- by find_lemmas_via_monom [real.archimedean, exists_rat_btwn]
