src/tactic/hammer/mex3.lean
@@ -1,0 +1,8 @@
+import tactic.hammer.monomorphization data.nat.gcd data.real.basic
+
+-- set_option profiler true
+set_option trace.super true
+
+example {α} [linear_ordered_field α] [archimedean α] {x y : α} (h : x < y) :
+  ∃ q : ℚ, x < q ∧ (q:α) < y :=
+by hammer_via_monom
