src/tactic/hammer/mex6.lean
@@ -1,0 +1,7 @@
+import tactic.hammer.monomorphization data.nat.gcd data.real.basic
+
+-- set_option profiler true
+set_option trace.super true
+
+example (x y : ℕ) : nat.gcd x y ∣ x :=
+by hammer_via_monom
