src/tactic/hammer/mex8.lean
@@ -1,0 +1,9 @@
+import tactic.hammer.monomorphization data.nat.gcd data.real.basic
+
+-- set_option profiler true
+set_option trace.super true
+example (x y : ℕ) : x ∣ x * y :=
+by hammer_via_monom
+-- by feature_search
+-- by find_lemmas_via_monom [dvd_mul_right]
+-- by find_lemmas_via_monom [dvd_mul_right, foo, foo'] -- [nat.gcd_dvd]
